\mychapter{1}{Lesson 1}

\section{Problems in Cryptography}

- Confidential communication 

\todo{Image of Alice,Bob, Eve in ske}

\textbf{Kerckhoffs's principle:} \underline{No security by obscurity.}

Security should only rely on the secrecy of the key. However sharing the key between two parties is a costly operation.

\textbf{Syntax:}
\begin{itemize}
    \item $\K = $ Key Space
    \item $\M = $ Message Space
    \item $\C = $ Ciphertext Space
    \item $Enc: \K \times \M \to \C$
    \item $Dec: \K \times \C \to \M$
\end{itemize}

\textbf{Correctness:}

$\forall m \in \M, \forall k \in \K : Dec(k, Enc(k,m))=m$

\begin{definition}
    Perfect Secrecy (SHANNON)

    Let M be any distribution over $\M$.

    Let K be uniform over $\K$.

    We say that $(Enc, Dec)$ is perfectly secret if $\forall M, \forall m \in \M, \forall c \in \C$.

    $$Pr[M=m]=Pr[M=m|C=c]$$
    Meaning that the ciphertext does not reveal anything about the message.
\end{definition}

\begin{theorem}
    Let M, K, C as above. The following are equivalent:
\end{theorem}

\begin{enumerate}[I]
    \item $Pr[M=m]=Pr[M=m|C=c]$
    \item M and C are INDEPENDENT
    \item $\forall m, m' \in \M, \forall c \in C$ $Pr[Enc(k,m)=c]=Pr[Enc(k,m')=c]$
\end{enumerate}

\begin{proof}

    $(I)\implies(II)$
    \begin{gather*}
        Pr[M=m \wedge C=c]=Pr[C=c]Pr[M=m|C=c]=Pr[C=c]Pr[M=m]   
    \end{gather*}
    They are independent.
    
    $(II)\implies(III)$
    Fix M, any $m\in M, c\in C$
    \begin{gather*}
        Pr[Enc(K,m)=c]=Pr[Enc(K,M)=c|M=m]=Pr[C=c|M=m]=Pr[C=c]   
    \end{gather*}

    $(III)\implies(I)$
    \begin{gather*}
        Pr[C=c]=\sum_{m'}Pr[C=c\wedge M=m']=\\
        =\sum_{m'}Pr[Enc(K,M)=c\wedge M=m']=\\
        =\sum_{m'}Pr[Enc(K,M)=c| M=m']Pr[M=m']=\\
        =\sum_{m'}Pr[Enc(K,m')=c]Pr[M=m']= \text{(Using III)}\\
        =Pr[Enc(K,m)=c]\underbrace{\sum_{m'}Pr[M=m']}_{=1}=\\
        =Pr[Enc(K,m)=c]=Pr[Enc(K,M)=c|M=m]=\\
        =\underbrace{Pr[C=c|M=m]}_{\text{\shortstack{The proof ends here\\but we want (I)}}}\implies Pr[M=m]Pr[C=c|M=m]\implies\\
        \implies P[M=m]=\frac{Pr[C=c]Pr[M=m|C=c]}{Pr[C=c|M=m]}\\
        \implies Pr[M=m]=Pr[M=m|C=c]
    \end{gather*}
\end{proof}

\todo{\section{One Time Pad}}
